\input{../header}
\input{mydef}


\usepackage{flowchart}
\usetikzlibrary{arrows}

\usepackage{natbib}
\bibliographystyle{plain}



\begin{document}

Generalised linear model may be presented in form
\[
L(\theta) = S^T \theta - A(\theta)
\]
where
\[
A(\theta) = \sum_i g(\psi_i^T \theta), 
\quad
S = \sum_i Y_i \psi_i.
\]
This model has following properties
\[
D^2 = \sum_i g''(\psi_i^T \theta) \psi_i \psi_i^T,
\quad
\delta(r) = a_g \delta_{\psi} r,
\quad  a_g = \max g'''/g'',
\quad \delta_{\psi} = \max_i \normp{D^{-1} \psi_i}.
\]
From condition (\ref{cond_A}) for likelihood function $L(\theta)$ one get
\[
\left |
\sqrt{2 \dLh(\opttheta, \opttheta_1, \opttheta_2)} - 
\normp{
\begin{matrix}
D_1(\opttheta - \opttheta_1) \\
D_2(\opttheta - \opttheta_2) \\
\end{matrix}}
\right |
\leq c_1 \delta(\sqrt{2}r).
\]
Find relation between $\opttheta, \opttheta_1, \opttheta_2$
\[
\normp{D (\opttheta - \theta)} \leq 
\normp{
D^{-1}\{ D_1 D_1^{-1}  \nabla L_1(\theta) + D_2 D_2^{-1} \nabla L_2(\theta) \}
} + c_2 \delta(r).
\]
\[
\normp{ D^{-1} D_1 \{ D_1^{-1}  \nabla L_1(\theta) -  D_1(\theta - \opttheta_1) \} } \leq c_3 \delta(r).
\]
\[
\normp{ D^{-1} D_2 \{ D_2^{-1}  \nabla L_2(\theta) -  D_2(\theta - \opttheta_2) \} } \leq c_3 \delta(r).
\]
Define vector $\widetilde{\theta}$ close to $\opttheta$
\[
\widetilde{\theta} = (D_1^2 + D_2^2)^{-1} (D_1^2 \opttheta_1 + D_2^2 \opttheta_2)
\]

\[
\left |
\normp{
\begin{matrix}
D_1(\opttheta - \opttheta_1) \\
D_2(\opttheta - \opttheta_2) \\
\end{matrix}}  - 
\normp{
\begin{matrix}
D_1(\widetilde{\theta} - \opttheta_1) \\
D_2(\widetilde{\theta}  - \opttheta_2) \\
\end{matrix}}
\right | 
\leq 
\normp{D (\opttheta - \widetilde{\theta})} 
\leq 
 c_2 \delta(r) +  c_3 \delta(\sqrt{2} r).
\]
\[
\normp{
\begin{matrix}
D_1(\widetilde{\theta} - \opttheta_1) \\
D_2(\widetilde{\theta}  - \opttheta_2) \\
\end{matrix}}  = 
\normp{D_{12} (\opttheta_2 - \opttheta_1)},
\quad D_{12} =  D_1 D^{-1} D_2.
\]
Temporary result is
\[
\left |
\sqrt{2 \dLh(\opttheta, \opttheta_1, \opttheta_2)} - 
\normp{D_{12} (\opttheta_2 - \opttheta_1)}
\right |
\leq c_1 \delta(\sqrt{2}r)  +  c_2 \delta(r) +  c_3 \delta(\sqrt{2} r).
\]
Involve $\xi_1$ and $\xi_2$  by means of Fisher theorem
\[
\normp{
\begin{matrix}
D_2 D^{-1} \{ D_1(\opttheta_1 - \theta^*_1 ) - \xi_1 \} \\
D_1 D^{-1} \{ D_2(\opttheta_2 - \theta^*_2 ) - \xi_2 \} \\
\end{matrix}} 
\leq
c_4 \delta(\sqrt{2} r).
\]
Finally,
\[
\left |
\sqrt{2 \dLh(\opttheta, \opttheta_1, \opttheta_2)} - 
\normp{D_{12} (\theta^*_2 - \theta^*_1) + \xi_{12}}
\right |
\leq c_1 \delta(\sqrt{2}r)  +  c_2 \delta(r) +  c_3 \delta(\sqrt{2} r) + c_4 \delta(\sqrt{2} r).
\]



\end{document}